Aux.v
@@ -1,0 +1,13 @@
+
+Require Import String.
+
+Fixpoint sofn (n : nat) : string :=
+match n with
+| 0 => "0"
+| S (S (S (S (S (S (S (S (S (S 0))))))))) => "X"
+| S (S (S (S (S (S (S (S (S (S n))))))))) => "X" ++ sofn n
+| S (S (S (S (S 0)))) => "V"
+| S (S (S (S (S n)))) => "V" ++ sofn n
+| S 0 => "i"
+| S n => "i" ++ sofn n
+end.
