PlanarLambda.v
@@ -1,0 +1,65 @@
+
+Require Import String.
+
+Require Import Aux.
+
+Inductive pterm : nat -> Type :=
+| PVar : pterm 1
+| PAbs {n} : pterm (S n) -> pterm n
+| PApp {n} {m} : pterm n -> pterm m -> pterm (n + m).
+
+Fixpoint s_of_pterm {k : nat} (i o : nat) (pt : pterm k) : nat * nat * string :=
+match pt with
+| PVar => (i, S o, sofn o)
+| PAbs pt' =>
+  match pt' with
+  | PVar =>
+    let s := ("L " ++ (sofn i) ++ "." ++ (sofn i))%string in
+    (S i, S o, s)
+  | PAbs _ =>
+    let (io', s') := s_of_pterm (S i) o pt' in
+    match s' with
+    | String _ s'' =>
+      let s := ("L " ++ (sofn i) ++ s'')%string in
+      (io', s)
+    | _ => (0, 0, ""%string)
+    end
+  | PApp _ _ =>
+    let (io', s') := s_of_pterm (S i) o pt' in
+    let s := ("L " ++ (sofn i) ++ ".(" ++ s' ++ ")")%string in
+    (io', s)
+  end
+| PApp pt1 pt2 =>
+  let (io1, s1) := s_of_pterm i o pt1 in
+  let (i1, o1) := io1 in
+  let (io2, s2) := s_of_pterm i1 o1 pt2 in
+  let s := match pt1 with
+  | PAbs _ => ("(" ++ s1 ++ ") " ++ s2)%string
+  | _ => (s1 ++ " " ++ s2)%string
+  end in
+  (io2, s)
+end.
+
+Definition sofpt {a : nat} (pt : pterm a) : string :=
+  let (_, s) := s_of_pterm 0 0 pt in s.
+
+Fixpoint sofpt' {k : nat} (pt : pterm k) : string :=
+match pt with
+| PVar => "v"
+| PAbs pt' =>
+  match pt' with
+  | PVar => "L.v"
+  | PAbs _ => "L" ++ sofpt' pt'
+  | PApp _ _ => "L.(" ++ sofpt' pt' ++ ")"
+  end
+| PApp pt1 pt2 =>
+  match pt1 with
+  | PAbs _ => "(" ++ sofpt' pt1 ++ ") " ++ sofpt' pt2
+  | _ => sofpt' pt1 ++ " " ++ sofpt' pt2
+  end
+end.
+
+Eval compute in sofpt (PAbs (PAbs (PApp PVar (PAbs (PApp PVar PVar))))).
+Eval compute in sofpt' (PAbs (PAbs (PApp PVar (PAbs (PApp PVar PVar))))).
+
+
