Snoclist.v
@@ -1,0 +1,51 @@
+
+Inductive snoclist (A : Type) : Type :=
+| nil : snoclist A
+| snoc : snoclist A -> A -> snoclist A.
+
+Arguments nil {A}.
+Arguments snoc {A} l a.
+
+Declare Scope snoclist_scope.
+Delimit Scope snoclist_scope with snoclist.
+Bind Scope snoclist_scope with snoclist.
+
+Open Scope snoclist_scope.
+
+Infix "::" := snoc (at level 60, right associativity) : snoclist_scope.
+
+Module SnoclistNotations.
+Notation "[ ]" := nil (format "[ ]"): snoclist_scope.
+Notation "[ x ]" := (snoc nil x): snoclist_scope.
+(*
+Notation "[ x ; y ; .. ; z ]" := (snoc (snoc .. (snoc nil x) .. y) z)
+  (format "[ '[' x ; '/' y ; '/' .. ; '/' z ']' ]"): snoclist_scope.
+*)
+End SnoclistNotations.
+
+Import SnoclistNotations.
+
+Definition length {A : Type} : snoclist A -> nat :=
+  fix length l :=
+  match l with
+   | nil => O
+   | l' :: _ => S (length l')
+  end.
+
+Definition app {A : Type} : snoclist A -> snoclist A -> snoclist A :=
+  fix app l m :=
+  match m with
+   | nil => l
+   | m' :: a => app l m' :: a
+  end.
+
+Infix "++" := app (right associativity, at level 60) : snoclist_scope.
+
+Section Facts.
+
+Variable A : Type.
+
+Theorem nil_snoc (x:A) (l:snoclist A) : [] <> l :: x.
+Admitted.
+
+End Facts.
