Types.v
@@ -1,0 +1,20 @@
+
+Require Import String.
+
+Require Import Aux.
+
+Inductive type : Type :=
+| TVar : nat -> type
+| TImp : type -> type -> type.
+
+Fixpoint softy (ty : type) : string :=
+match ty with
+| TVar n => sofn n
+| TImp ty1 ty2 =>
+  match (ty1, ty2) with
+  | (TVar n, TVar m) => sofn n ++ " -> " ++ sofn m
+  | (TVar n, _) => sofn n ++ " -> " ++ softy ty2
+  | (_, TVar m) => "(" ++ softy ty1 ++ ") -> " ++ sofn m 
+  | _ => "(" ++ softy ty1 ++ ") -> " ++ softy ty2
+  end
+end.
