Workbench.v
@@ -1,0 +1,20 @@
+
+Require Import Snoclist.
+Import SnoclistNotations.
+Require Import PlanarLambda.
+Require Import Types.
+
+Definition context : Type := snoclist type.
+
+Inductive test (n : nat) (pt : pterm n) : Type :=
+| Test : test n pt.
+
+Inductive test2 : nat -> Type :=
+| Test2 : test2 0.
+
+Check test2.
+
+(*
+Inductive is_typed : context -> pterm (a : nat) -> type -> Prop :=
+| type_var ty : is_typed [ty] PVar ty.
+*)
